sketch intermediate game after first reduction (eexpRev replaces H1)

examples/AKE/AKE_proof.ec
@@ -211,50 +211,236 @@ module AKE(FA : Adv) = {
   }
 }.
 
-
 pred test_fresh(t : Sid option, evs : Event list) =
   t <> None /\ fresh (proj t) evs.
 
 (*{ Explain security notion *)
 section.
-  (* For an arbitrary adversary A, *)
-  declare module A : Adv.
-
-  (* we want to a find (small) bound eps *)
+  (* We want to a find (small) bound eps *)
   const eps : real.
 
-  (* such that the advantage of the adversary is upper bounded by eps. *)
+  (* such that the advantage of an adversary is upper bounded by eps. *)
   axiom Secure:
-    forall &m,
+    forall (A <: Adv) &m,
       2%r * Pr[   AKE(A).main() @ &m : res /\ test_fresh AKE.test AKE.evs] - 1%r < eps.
 end section.
 (*} end: Explain security notion *)
 
 (*} end: Initial game and security definition *)
 
-lemma Eq_G0_G0_1_1:
-  forall (A <: Adv),
-    equiv[  AKE(A).main ~ G0_1_0(A).main
-          : true ==> ={res} /\ (test_fresh AKE.test AKE.evs){1} = 
-                               (test_fresh G0_1_0.test G0_1_0.evs){2}].
-proof strict.
-  intros=> A.
-  fun. inline RO_H1.LRO.init.
-  swap {1} 9 7. swap {2} 9 7.
-  seq 6 6:
-    (={pks,b',i} /\
-     AKE.mSk{1} = G0_1.mSk{2} /\
-     AKE.cSession{1} = G0_1.cSession{1}).
-(*     AKE.cH1{1} = G0_1.cH1{2} /\
-     AKE.cH2{1} = G0_1.cH2{2} /\
-   (*  AKE.mH1{1} = RO_H1.LRO.m{2} /\ *)
-     AKE.sH1{1} = G0_1.sH1{2} /\
-     AKE.mH2{1} = G0_1.mH2{2} /\
-     AKE.sH2{1} = G0_1.sH2{2} /\
-     AKE.mStarted{1} = G0_1.mStarted{2} /\
-     AKE.mCompleted{1} =  G0_1.mCompleted{2} /\
-     AKE.evs{1} = G0_1.evs{2} /\
-     AKE.test{1} = G0_1.test{2}
-*)
-  eqobs_in. admit.
+(*{ First reduction: replace H1_A by EexpRev oracle *)
 
+module type AKE_Oracles2 = {
+  fun eexpRev(i : Sidx, a : Sk) : Eexp option
+  fun h2_a(sstring : Sstring) : Key option
+  fun init1(i : Sidx, A : Agent, B : Agent) : Epk option
+  fun init2(i : Sidx, Y : Epk) : unit
+  fun resp(i : Sidx, B : Agent, A : Agent, X : Epk) : Epk option
+  fun staticRev(A : Agent) : Sk option
+  fun sessionRev(i : Sidx) : Key option
+}.
+
+module type Adv2 (O : AKE_Oracles2) = {
+  fun choose(s : Pk list) : Sidx {*}
+  fun guess(k : Key option) : bool
+}.
+
+type Sdata2 = (Agent * Agent * Role).
+
+op sd2_actor(sd : Sdata2) = let (A,B,r) = sd in A.
+op sd2_peer(sd : Sdata2)  = let (A,B,r) = sd in B.
+op sd2_role(sd : Sdata2)  = let (A,B,r) = sd in r.
+
+op compute_sid(mStarted : (Sidx, Sdata2) map) (mEexp : (Sidx, Eexp) map)
+              (mCompleted : (Sidx, Epk) map) (i : Sidx) : Sid =
+  let (A,B,r) = proj mStarted.[i] in
+  (A,B,gen_epk(proj mEexp.[i]),proj mCompleted.[i],r).
+
+module AKE_EexpRev(FA : Adv2) = {
+  
+  var evs  : Event list               (* events for queries performed by adversary *)
+  var test : Sid option               (* session id of test session *)
+
+  var cSession, cH1, cH2 : int        (* counters for queries *)
+
+  var mH2 : (Sstring, Key) map        (* map for h2 *)
+  var sH2 : Sstring set               (* adversary queries for h2 *)
+
+  var mSk        : (Agent, Sk) map    (* map for static secret keys *)
+  var mEexp      : (Sidx, Eexp) map   (* map for ephemeral exponents of sessions *)
+  var mStarted   : (Sidx, Sdata2) map (* map of started sessions *)
+  var mCompleted : (Sidx, Epk)   map  (* additional data for completed sessions *)
+  
+  module O : AKE_Oracles2 = {
+    
+    fun eexpRev(i : Sidx, a : Sk) : Eexp option = {
+      var r : Eexp option = None;
+      if (in_dom i mStarted) {
+        evs = EphemeralRev(compute_sid mStarted mEexp mCompleted i)::evs;
+        if (sd2_actor(proj mStarted.[i]) = gen_pk(a)) {
+          r = mEexp.[i];
+        }
+      }
+      return r;
+    }
+    
+    fun h2(sstring : Sstring) : Key = {
+      var ke : Key;
+      ke = $sample_Key;
+      if (!in_dom sstring mH2) {
+        mH2.[sstring] = ke;
+      }
+      return proj mH2.[sstring];
+    }
+ 
+    fun h2_a(sstring : Sstring) : Key option = {
+      var r : Key option = None;
+      var ks : Key;
+      if (cH2 < qH2) {
+        cH2 = cH2 + 1;
+        sH2 = add sstring sH2;
+        ks = h2(sstring);
+        r = Some(ks);
+      }
+      return r;
+    }
+
+    fun init1(i : Sidx, A : Agent, B : Agent) : Epk option = {
+      var pX : Epk;
+      var r : Epk option = None; 
+      if (cSession < qSession && in_dom A mSk && in_dom B mSk && !in_dom i mStarted) {
+        cSession = cSession + 1;
+        pX = gen_epk(proj mEexp.[i]);
+        mStarted.[i] = (A,B,init);
+        evs = Start((A,B,pX,init))::evs;
+        r = Some(pX);
+      }
+      return r;
+    }
+
+    fun resp(i : Sidx, B : Agent, A : Agent, X : Epk) : Epk option = {
+      var pY : Epk;
+      var r : Epk option = None; 
+      if (   cSession < qSession && in_dom A mSk && in_dom B mSk
+          && !in_dom i mStarted && !in_dom i mCompleted) {
+        cSession = cSession + 1;
+        pY = gen_epk(proj mEexp.[i]);
+        mStarted.[i] = (B,A,resp);
+        mCompleted.[i] = X;
+        evs = Accept((B,A,pY,X,resp))::evs;
+        r = Some(pY);
+      }
+      return r;
+    }
+
+    fun init2(i : Sidx, Y : Epk) : unit = {
+      if (!in_dom i mCompleted && in_dom i mStarted) {
+        mCompleted.[i] = Y;
+        evs = Accept(compute_sid mStarted mEexp mCompleted i)::evs;
+      }
+    }
+
+    fun staticRev(A : Agent) : Sk option = {
+      var r : Sk option = None;
+      if (in_dom A mSk) {
+        r = mSk.[A];
+        evs = StaticRev(A)::evs;
+      }
+      return r;
+    }
+
+    fun computeKey(i : Sidx) : Key option = {
+      var r : Key option = None;
+      var a : Agent;
+      var b : Agent;
+      var ro : Role;
+      var x' : Eexp;
+      var x : Esk;
+      var k : Key;
+      if (in_dom i mCompleted) {
+        (a,b,ro) = proj mStarted.[i];
+        k = h2(gen_sstring (proj mEexp.[i]) (proj mSk.[a]) b (proj mCompleted.[i]) ro);
+        r = Some k;
+      }
+      return r;
+    }
+
+    fun sessionRev(i : Sidx) : Key option = {
+      var r : Key option = None;
+      if (in_dom i mCompleted) {
+        evs = SessionRev(compute_sid mStarted mEexp mCompleted i)::evs;
+        r = computeKey(i);
+      }
+      return r;
+    }
+  }
+  
+  module A = FA(O)
+
+  fun main() : bool = {
+    var b : bool;
+    var pks : Pk list = [];
+    var t_idx : Sidx;
+    var key : Key;
+    var keyo : Key option;
+    var b' : bool = false;
+    var i : int = 0;
+    var ska : Sk;
+    var pka : Pk;
+    var xa' : Eexp;
+
+    mSk = Map.empty;
+    while (i < qAgent) {
+      ska = $sample_Sk;
+      pka = gen_pk(ska);
+      pks = pka :: pks;
+      mSk.[pka] = ska;
+    }
+    
+    mEexp = Map.empty;
+    i = 0;
+    while (i < qSession) {
+      xa' = $sample_Eexp;
+      mEexp.[i] = xa';
+    } 
+
+    cSession = 0;
+    cH1 = 0;
+    cH2 = 0;
+    mH2 = Map.empty;
+    sH2 = FSet.empty;
+    mStarted = Map.empty;
+    mCompleted = Map.empty;
+    evs = [];
+    test = None;
+
+    t_idx = A.choose(pks);
+    b = ${0,1};
+    if (mStarted.[t_idx] <> None && mCompleted.[t_idx] <> None) {
+      test = Some (compute_sid mStarted mEexp mCompleted t_idx);
+        (* the if-condition implies "mem (Accept (proj O.test)) O.evs" *)
+      if (b) {
+        keyo = O.computeKey(t_idx);
+      } else {
+        key  = $sample_Key;
+        keyo = Some key;
+      }
+      b' = A.guess(keyo);
+    }
+    return (b = b');
+  }
+}.
+
+pred no_collision(m : (int, Eexp) map) =
+  ! (exists i j, in_dom i m /\ m.[i] = m.[j] /\ i <> j).
+
+section.
+  (* At this point, we still have to show the following: *)
+  axiom Remaining_obligation:
+    forall (A <: Adv2) &m,
+      2%r * Pr[ AKE_EexpRev(A).main() @ &m : res
+                    /\ test_fresh AKE_EexpRev.test AKE_EexpRev.evs
+                    /\ no_collision(AKE_EexpRev.mEexp) ] - 1%r < eps.
+end section.
+
+(*} *)
